VCG_test.v
@@ -1,0 +1,101 @@
+Require Import GPUCSL.
+Require Import VCG_refined.
+Require Import scan_lib.
+Section sum_of_number.
+Notation X := (Var "x").
+Notation T := (Var "t").
+Variable n : nat.
+
+Fixpoint sum n := match n with
+  | O => 0
+  | S n => Z.succ (Z.of_nat n) + sum n
+end%Z.
+Require Import Psatz.
+Lemma sum_Snn_2 (m : nat) : 
+  ((Z.of_nat m * (Z.of_nat m + 1)) / 2 = sum m)%Z.
+Proof.
+  induction m; [simpl; auto|].
+  cutrewrite (Zn (S m) * (Zn (S m) + 1) = Zn m * (Zn m + 1) + ((Zn m) + 1) * 2)%Z; [|nia].
+  rewrite Z.div_add; try omega.
+  rewrite IHm; simpl; omega.
+Qed.
+
+Import ListNotations.
+Open Scope list_scope.
+
+Require Import LibTactics.
+Program Definition INV :=
+  ex_ast _ (fun x : val => ex_ast _ (fun t : val => pure_ast (
+    {| Aenv := (X, x) :: (T, t) :: nil;
+       Aenv_wf := _;
+       Ap := (0 <= x /\ x <= Zn n /\ t = sum (Z.to_nat x))%Z;
+       sp := nil
+    |}))).
+Next Obligation.
+repeat split; jauto.
+intros [H | H]; jauto.
+congruence.
+Qed.
+
+Definition SUM :=
+  T ::= Enum' 0 ;;
+  X ::= Enum' 0 ;;
+  while (INV) (X < Enum' n) (
+    X ::= X + Enum 1 ;;
+    T ::= (T + X))%exp.
+
+Variable ntrd : nat.
+Variable tid : Fin.t ntrd.
+
+Lemma nil_wf : env_wf nil.
+simpl; eauto.
+Qed.
+
+Lemma one_wf x v : env_wf ((x, v) :: nil).
+simpl; eauto.
+Qed.
+
+Arguments exAst_denote : simpl never.
+Arguments Ast_denote : simpl never.
+
+Hint Unfold exAst_denote Ast_denote.
+
+Goal
+  CSL (fun _ => default ntrd) tid
+  (Ast_denote {| Aenv := nil;
+                 Aenv_wf := nil_wf;
+                 Ap := True;
+                 sp := nil|})
+  SUM 
+  (Ast_denote {| Aenv := (T, (sum n)) :: nil;
+                 Aenv_wf := one_wf _ _;
+                 Ap := True;
+                 sp := nil|}).
+Proof.
+  unfold SUM, INV; eapply Hforward.
+  repeat (sym_exec; [reflexivity|]).
+  sym_exec; [unfold INV; simpl; auto|..].
+  { unfold INV; autounfold; simpl; intros s h Hsat.
+    exists 0%Z 0%Z.
+    sep_split_in Hsat; sep_split; eauto.
+    destruct HP as ((? & ? & _) & _); repeat split; eauto; omega. }
+  simpl; sym_exec; intros x; sym_exec; intros t.
+  sym_exec; [reflexivity|].
+  simpl; eapply Hforward; [sym_exec; reflexivity |].
+  { autounfold in *; simpl in *; intros s h Hsat.
+    exists (x + 1)%Z (t + (x + 1))%Z.
+    sep_split; sep_split_in Hsat; eauto.
+    destruct HP as ((? & ? & _) & (? & ? & ? & ?)); repeat split; eauto; try omega.
+    cutrewrite (Z.to_nat (x + 1) = S (Z.to_nat x)); [|].
+    simpl; unfold val in *; rewrite Z2Nat.id; omega.
+    unfold val in *; rewrite Z2Nat.inj_add; simpl; nia. }
+  intros s h (x & t & Hsat); repeat (autounfold in *; simpl in *).
+  sep_split_in Hsat; sep_split; eauto.
+  destruct HP as ((? & ? & ?) & (? & ? & ? & ?)); repeat split; eauto; try omega.
+  unfold_conn_all; simpl in *; subst.
+  cutrewrite (n = Z.to_nat (s X)); eauto.
+  cutrewrite (s X = Zn n)%Z; [|omega].
+  rewrite Nat2Z.id; eauto.
+Qed.
+
+Section sum_of_number.
